common/Smallstep.v
@@ -528,7 +528,7 @@ Section FSIM.
 
 Context {liA1 liA2} (ccA: callconv liA1 liA2).
 Context {liB1 liB2} (ccB: callconv liB1 liB2).
-Context (se1 se2: Genv.symtbl) (wB: ccworld ccB).
+Context (se1 se2: Genv.symtbl) (se_path: Genv.symtbl_path se1 se2) (wB: ccworld ccB).
 Context {state1 state2: Type}.
 
 (** The general form of a forward simulation. *)
@@ -547,7 +547,7 @@ Record fsim_properties (L1: lts liA1 liB1 state1) (L2: lts liA2 liB2 state2) (in
       exists r2, final_state L2 s2 r2 /\ match_reply ccB wB r1 r2;
     fsim_match_external:
       forall i s1 s2 q1, match_states i s1 s2 -> at_external L1 s1 q1 ->
-      exists w q2, at_external L2 s2 q2 /\ match_query ccA w q1 q2 /\ match_senv ccA w se1 se2 /\
+      exists w q2, at_external L2 s2 q2 /\ match_query ccA w q1 q2 /\ match_senv ccA w se_path /\
       forall r1 r2 s1', match_reply ccA w r1 r2 -> after_external L1 s1 r1 s1' ->
       exists i' s2', after_external L2 s2 r2 s2' /\ match_states i' s1' s2';
     fsim_simulation:
@@ -602,7 +602,7 @@ Hypothesis match_final_states:
 
 Hypothesis match_external:
   forall s1 s2 q1, match_states s1 s2 -> at_external L1 s1 q1 ->
-  exists wA q2, at_external L2 s2 q2 /\ match_query ccA wA q1 q2 /\ match_senv ccA wA se1 se2 /\
+  exists wA q2, at_external L2 s2 q2 /\ match_query ccA wA q1 q2 /\ match_senv ccA wA se_path /\
   forall r1 r2 s1', match_reply ccA wA r1 r2 -> after_external L1 s1 r1 s1' ->
   exists s2', after_external L2 s2 r2 s2' /\ match_states s1' s2'.
 
@@ -638,8 +638,10 @@ Proof.
 - intros. exploit match_initial_states; eauto. intros [s2 [A B]].
     exists s1; exists s2; auto.
 - intros. destruct H. eapply match_final_states; eauto.
-- intros. destruct H. edestruct match_external as (w & q2 & H2 & Hq & Hw & Hr); eauto.
-  exists w, q2. intuition auto. edestruct Hr as (s2' & Hs2' & Hs'); eauto.
+- intros. destruct H.
+  edestruct match_external as (wA & q2 & H2 & Hq & Hw & Hr); eauto.
+  exists wA, q2. intuition auto.
+  edestruct Hr as (s2' & Hs2' & Hs'); eauto.
 - intros. destruct H0. subst i. exploit simulation; eauto. intros [s2' [A B]].
   exists s1'; exists s2'; intuition auto.
 Qed.
@@ -812,20 +814,21 @@ End SIMULATION_SEQUENCES.
 
 End FSIM.
 
-Arguments fsim_properties {_ _} _ {_ _} _ _ _ _ {_ _} L1 L2 index order match_states.
+Arguments fsim_properties {_ _} _ {_ _} _ {_ _} _ _ {_ _} L1 L2 index order match_states.
 
-Record fsim_components {liA1 liA2} (ccA: callconv liA1 liA2) {liB1 liB2} ccB L1 L2 :=
+Record fsim_components {liA1 liA2} (ccA: callconv liA1 liA2)
+  {liB1 liB2} (ccB: callconv liB1 liB2) L1 L2 :=
   Forward_simulation {
     fsim_index: Type;
     fsim_order: fsim_index -> fsim_index -> Prop;
     fsim_match_states: _;
 
     fsim_skel:
-      skel L1 = skel L2;
-    fsim_lts se1 se2 wB:
-      @match_senv liB1 liB2 ccB wB se1 se2 ->
-      Genv.valid_for (skel L1) se1 ->
-      fsim_properties ccA ccB se1 se2 wB (activate L1 se1) (activate L2 se2)
+      Genv.skel_path (skel L1) (skel L2);
+    fsim_lts se1 se2 (se_path: Genv.symtbl_path se1 se2) wB:
+      match_senv ccB wB se_path ->
+      Genv.valid_stbls fsim_skel se_path ->
+      fsim_properties ccA ccB se_path wB (activate L1 se1) (activate L2 se2)
         fsim_index fsim_order (fsim_match_states se1 se2 wB);
     fsim_order_wf:
       well_founded fsim_order;
@@ -835,30 +838,6 @@ Arguments Forward_simulation {_ _ ccA _ _ ccB L1 L2 fsim_index}.
 
 Definition forward_simulation {liA1 liA2} ccA {liB1 liB2} ccB L1 L2 :=
   inhabited (@fsim_components liA1 liA2 ccA liB1 liB2 ccB L1 L2).
-
-
-Record fsim_components' {liA1 liA2} (ccA: callconv liA1 liA2) {liB1 liB2} ccB L1 L2 :=
-  Forward_simulation' {
-    fsim_index': Type;
-    fsim_order': fsim_index' -> fsim_index' -> Prop;
-    fsim_match_states': _;
-
-    fsim_skel':
-      Genv.skel_le (skel L2) (skel L1);
-    fsim_lts' se1 se2 wB:
-      @match_senv liB1 liB2 ccB wB se1 se2 ->
-      Genv.skel_symtbl_compatible (skel L1) (skel L2) se1 se2 ->
-      fsim_properties ccA ccB se1 se2 wB (activate L1 se1) (activate L2 se2)
-        fsim_index' fsim_order' (fsim_match_states' se1 se2 wB);
-    fsim_order_wf':
-      well_founded fsim_order';
-  }.
-
-Arguments Forward_simulation' {_ _ ccA _ _ ccB L1 L2 fsim_index'}.
-
-Definition forward_simulation' {liA1 liA2} ccA {liB1 liB2} ccB L1 L2 :=
-  inhabited (@fsim_components' liA1 liA2 ccA liB1 liB2 ccB L1 L2).
-
 
 (** ** Tactics for forward simulation proofs *)
 
@@ -892,11 +871,18 @@ Tactic Notation (at level 3) "fsim" tactic3(tac) := fsim_tac tac.
 
 (** ** Identity simulation *)
 
+Existing Instance Genv.skel_le_refl.
+Existing Instance Genv.skel_le_tran.
+
 Definition identity_fsim_components {liA liB} (L: semantics liA liB):
   fsim_components cc_id cc_id L L.
 Proof.
-  eapply Forward_simulation with _ (fun _ _ _ => _); auto.
-  - intros se _ [ ] [ ] _.
+  (* eapply Forward_simulation. *)
+  (* instantiate (1 := (fun _ _ _ => _)). *)
+  assert (path: Genv.skel_path (skel L) (skel L)).
+  { eapply Genv.Direct. reflexivity. }
+  eapply Forward_simulation with _ (fun _ _ _ => _) path; auto.
+  - intros se ? se_path w Hse Hvs. inv Hse. destruct w.
     eapply forward_simulation_plus with (match_states := eq);
     cbn; intros; subst; eauto 10 using plus_one.
     exists tt, q1. intuition (subst; eauto).
@@ -917,13 +903,16 @@ Context {liA1 liA2 liA3} {ccA12: callconv liA1 liA2} {ccA23: callconv liA2 liA3}
 Context {liB1 liB2 liB3} {ccB12: callconv liB1 liB2} {ccB23: callconv liB2 liB3}.
 Context (L1: semantics liA1 liB1) (L2: semantics liA2 liB2) (L3: semantics liA3 liB3).
 
+Require Import Coq.Program.Equality.
+
 Lemma compose_fsim_components:
   fsim_components ccA12 ccB12 L1 L2 ->
   fsim_components ccA23 ccB23 L2 L3 ->
   fsim_components (ccA12 @ ccA23) (ccB12 @ ccB23) L1 L3.
 Proof.
-  intros [index order match_states Hsk props order_wf].
-  intros [index' order' match_states' Hsk' props' order_wf'].
+  intros [index order match_states path12 props order_wf].
+  intros [index' order' match_states' path23 props' order_wf'].
+  set (sk2 := skel L2).
   set (ff_index := (index' * index)%type).
   set (ff_order := lex_ord (clos_trans _ order') order).
   set (ff_match_states :=
@@ -931,12 +920,18 @@ Proof.
            exists s2,
              match_states se1 se2 w (snd i) s1 s2 /\
              match_states' se2 se3 w' (fst i) s2 s3).
-  apply Forward_simulation with ff_order ff_match_states.
-  3: { unfold ff_order. auto using wf_lex_ord, wf_clos_trans. }
-  1: { congruence. }
-  intros se1 se3 [[se2 w] w'] (Hse12 & Hse23) Hse1. cbn in *.
-  assert (Hse2: Genv.valid_for (skel L2) se2).
-  { rewrite <- Hsk. eapply match_senv_valid_for; eauto. }
+  apply Forward_simulation
+    with ff_order ff_match_states (Genv.Compose path12 path23).
+  2: { unfold ff_order. auto using wf_lex_ord, wf_clos_trans. }
+
+  intros se1 se3 se_path13 [[se2 w] w'] Hse Hvs. cbn in *.
+  simple inversion Hvs; subst. { exfalso. inv H1. }
+  dependent destruction H1.
+  simple inversion Hse. 2: { exfalso. inv H0. } inv H.
+  dependent destruction H0.
+  intros Hse12 Hse23 Hvs12 Hvs23.
+  clear Hvs Hse. rename se12 into se2.
+
   constructor.
 - (* valid query *)
   intros q1 q3 (q2 & Hq12 & Hq23).
@@ -956,6 +951,7 @@ Proof.
   edestruct (@fsim_match_external liA1) as (w12 & q2 & Hq2 & Hq12 & Hw12 & Hk12); eauto.
   edestruct (@fsim_match_external liA2) as (w23 & q3 & Hq3 & Hq23 & Hw23 & Hk23); eauto.
   exists (se2, w12, w23), q3. cbn; repeat apply conj; eauto.
+  { constructor; eauto. }
   intros r1 r3 s1' (r2 & Hr12 & Hr23) Hs1'.
   edestruct Hk12 as (i12' & s2' & Hs2' & Hs12'); eauto.
   edestruct Hk23 as (i23' & s3' & Hs3' & Hs23'); eauto.
